theories/Extraction/Subtyping.v
@@ -1,0 +1,113 @@
+From Mcltt Require Import Base LibTactics.
+From Mcltt.Algorithmic Require Import Subtyping.Definitions.
+From Mcltt.Core Require Import NbE.
+From Mcltt.Extraction Require Import Evaluation NbE.
+From Equations Require Import Equations.
+Import Domain_Notations.
+
+
+#[local]
+  Ltac subtyping_tac :=
+  lazymatch goal with
+  | |- {{ ⊢anf ~_ ⊆ ~_ }} =>
+      subst;
+      mauto 4;
+      try congruence;
+      econstructor; simpl; trivial
+  | |- ~ {{ ⊢anf ~_ ⊆ ~_ }} =>
+      let H := fresh "H" in
+      intro H; dependent destruction H; simpl in *;
+      try lia;
+      try congruence
+  end.
+
+#[tactic="subtyping_tac"]
+Equations subtyping_nf_impl A B : { {{ ⊢anf A ⊆ B }} } + {~ {{ ⊢anf A ⊆ B }} } :=
+| n{{{ Type@i }}}, n{{{ Type@j }}} with Compare_dec.le_lt_dec i j => {
+  | left _ => left _;
+  | right _ => right _
+  }
+| n{{{ Π A B }}}, n{{{ Π A' B' }}} with nf_eq_dec A A' => {
+  | left _ with subtyping_nf_impl B B' => {
+    | left _ => left _
+    | right _ => right _
+    }
+  | right _ => right _
+  }
+| A, B with nf_eq_dec A B => {
+  | left _ => left _
+  | right _ => right _
+  }.
+
+Theorem subtyping_nf_impl_complete : forall A B,
+    {{ ⊢anf A ⊆ B }} ->
+    exists H, subtyping_nf_impl A B = left H.
+Proof.
+  intros; dec_complete.
+Qed.
+
+
+Inductive subtyping_order G A B :=
+| subtyping_order_run :
+  nbe_ty_order G A ->
+  nbe_ty_order G B ->
+  subtyping_order G A B.
+#[local]
+  Hint Constructors subtyping_order : mcltt.
+
+
+Lemma subtyping_order_sound : forall G A B,
+    {{ G ⊢a A ⊆ B }} ->
+    subtyping_order G A B.
+Proof.
+  intros * H.
+  dependent destruction H.
+  mauto using nbe_ty_order_sound.
+Qed.
+
+#[local]
+  Ltac subtyping_impl_tac1 :=
+  match goal with
+  | H : subtyping_order _ _ _ |- _ => progressive_invert H
+  | H : nbe_ty_order _ _ |- _ => progressive_invert H
+  end.
+
+#[local]
+  Ltac subtyping_impl_tac :=
+  repeat subtyping_impl_tac1; try econstructor; mauto.
+
+
+#[tactic="subtyping_impl_tac"]
+Equations subtyping_impl G A B (H : subtyping_order G A B) :
+  { {{G ⊢a A ⊆ B}} } + { ~ {{ G ⊢a A ⊆ B }} } :=
+| G, A, B, H =>
+    let (a, Ha) := nbe_ty_impl G A _ in
+    let (b, Hb) := nbe_ty_impl G B _ in
+    match subtyping_nf_impl a b with
+    | left _ => left _
+    | right _ => right _
+    end.
+Next Obligation.
+  progressive_inversion.
+  functional_nbe_rewrite_clear.
+  contradiction.
+Qed.
+
+
+Theorem subtyping_impl_complete' : forall G A B,
+    {{G ⊢a A ⊆ B}} ->
+    forall (H : subtyping_order G A B),
+      exists H', subtyping_impl G A B H = left H'.
+Proof.
+  intros; dec_complete.
+Qed.
+
+#[local]
+ Hint Resolve subtyping_order_sound subtyping_impl_complete' : mcltt.
+
+Theorem subtyping_impl_complete : forall G A B,
+    {{G ⊢a A ⊆ B}} ->
+    exists H H', subtyping_impl G A B H = left H'.
+Proof.
+  repeat unshelve mauto.
+Qed.
